\section{Fractions}
\begin{center}
    \begin{longtable}{lcr}
        $\frac{a}{b} \pm \frac{c}{d} = \frac{a \cdot d \pm c \cdot b}{b \cdot d}$
        &
        $\frac{a}{b} \cdot \frac{c}{d} = \frac{a \cdot c}{b \cdot d}$
        &
        $c \cdot \frac{a}{b} = \frac{c \cdot a}{b}$
        \\
        $\frac{a}{c} \pm \frac{b}{c} = \frac{a \pm b}{c}$
        &
        $\frac{a}{b} = \frac{\frac{a}{c}}{\frac{b}{c}}$
        &
        $\frac{a}{b} = \frac{a \cdot c}{b \cdot c}$
        \\
        $a = \frac{a}{1}$
        &
        $\sqrt{\frac{a}{b}} = \frac{\sqrt{a}}{\sqrt{b}}$
        &
        $\left(\frac{a}{b}\right)^n = \frac{a^n}{b^n}$
        \\
        $\frac{\frac{a}{b}}{\frac{c}{d}} = \frac{a}{b} \cdot \frac{d}{c}$
        &
        $\frac{\frac{a}{b}}{c} = \frac{a}{b \cdot c}$
        &
        $\frac{a}{\frac{b}{c}} = \frac{a \cdot c}{b}$
        \\
        $-\frac{a}{b} = \frac{-a}{b} = \frac{a}{-b}$
        &
        $\frac{-a}{-b} = \frac{a}{b}$
        &
        $\frac{1}{a} = a^{-1}$
        \\
        $\frac{a}{a} = 1$
        &
        $\frac{a}{c} \cdot \frac{c}{b} = \frac{a}{b}$
        &
        $\frac{a}{b} \cdot b = a$
        \\
        $a \pm \frac{b}{c} = \frac{a \cdot c \pm b}{c}$
        &
        $\frac{b}{c} - a = \frac{b - a \cdot c}{c}$
    \end{longtable}
\end{center}
